lib/Algebra.v
@@ -1,0 +1,156 @@
+(*TODO: fix imports to reduce duplication*)
+Require Import Task.
+Require Import Theory.
+Require Import Typechecker.
+Require Import Tactics.
+Require Import Notations.
+From mathcomp Require Import all_ssreflect.
+Set Bullet Behavior "Strict Subproofs".
+
+(*TODO: maybe change TheoryTest, see*)
+
+(*TODO: different than other version because we use [funsym_noty]
+  instead of writing manually*)
+Definition const name ty := funsym_noty name nil ty.
+Definition binop name ty : funsym := funsym_noty name [ty;ty] ty.
+Definition unop name ty : funsym := funsym_noty name [ty] ty.
+
+Module Algebra.
+Local Open Scope string_scope.
+Local Open Scope why3_scope.
+
+(*Generic definitions*)
+Definition t_ts : typesym := mk_ts "t" nil.
+Definition t : vty := vty_cons t_ts nil.
+
+(*TODO: move, make more general*)
+Definition op: funsym := binop "op" t. 
+Definition unit : funsym := const "Unit" t.
+
+Definition inv : funsym := unop "inv" t. 
+(*Definition op (t1 t2: term) : term :=
+  Tfun op_fs nil [t1; t2].*)
+
+Definition x : vsymbol := ("x"%string, t).
+Definition y : vsymbol := ("y"%string, t).
+Definition z : vsymbol := ("z"%string, t).
+
+Coercion Tvar : vsymbol >-> term.
+
+(*TODO: the brackets for variables are ugly, but Coq will not convert appropriately*)
+
+(*Associativity*)
+Definition Assoc : theory :=
+  rev [
+    tdef (abs_type t_ts);
+    tdef (abs_fun op);
+    tprop Paxiom "Assoc"
+      <f forall x y z, 
+        [t] (op (op ({x}, {y}), {z})) = (op ({x}, (op({y}, {z})))) f>
+  ].
+
+(*Commutativity*)
+Definition Comm : theory :=
+  rev [
+    tdef (abs_type t_ts);
+    tdef (abs_fun op);
+    tprop Paxiom "Comm" <f
+     forall x y, [t] op({x}, {y}) = op({y}, {x}) f>
+  ].
+
+(*Associativity and Commutativity*)
+Definition AC : theory :=
+  rev [
+    tclone Assoc None nil nil nil;
+    tclone Comm None [(t_ts, t_ts)] [(op, op)] nil
+  ].
+
+(*Monoids*)
+Definition Monoid : theory :=
+  rev [
+    tclone Assoc None nil nil nil;
+    tdef (abs_fun unit);
+    tprop Paxiom "Unit_def_l" <f
+      forall x, [t] op (unit(), {x}) = {x} f>
+  ].
+
+(*Commutative monoids*)
+Definition CommutativeMonoid : theory :=
+  rev [
+    tclone Monoid None nil nil nil;
+    tclone Comm None [(t_ts, t_ts)] [(op, op)] nil
+  ].
+
+(*Groups*)
+Definition Group : theory :=
+  rev [
+    tclone Monoid None nil nil nil;
+    tdef (abs_fun inv);
+    tprop Paxiom "Inv_def_l" <f
+      forall x, [t] op (inv({x}), {x}) = unit() f>;
+    tprop Paxiom "Inv_def_r" <f
+      forall x, [t] op ({x}, inv({x})) = unit() f>
+  ].
+
+(*Commutative groups*)
+Definition CommutativeGroup : theory :=
+  rev [
+    tclone Group None nil nil nil;
+    tclone Comm None [(t_ts, t_ts)] [(op, op)] nil
+  ].
+
+(*Rings*)
+Definition zero : funsym := const "zero" t.
+Definition plus : funsym := binop "plus" t.
+Definition mult : funsym := binop "mult" t.
+Definition neg : funsym := unop "neg" t.
+(*Qualified names - TODO: improve*)
+Definition MA_t_ts : typesym := mk_ts "MulAssoc.t" nil.
+Definition MA_t : vty := vty_cons MA_t_ts nil.
+Definition MA_op: funsym := binop "MulAssoc.op" MA_t.
+
+(*We do not support infix notation*)
+Definition Ring : theory :=
+  rev [
+    tdef (abs_type t_ts);
+    tdef (abs_fun zero);
+    tdef (abs_fun plus);
+    tdef (abs_fun neg);
+    tdef (abs_fun mult);
+    tclone CommutativeGroup None [(t_ts, t_ts)] 
+      [(unit, zero); (op, plus); (inv, neg)] nil;
+    tclone Assoc (Some "MulAssoc")  [(MA_t_ts, t_ts)] [(MA_op, mult)] nil;
+    tprop Paxiom "Mul_distr_l" <f
+      forall x y z, [t] mult({x}, plus({y}, {z})) = plus(mult({x}, {y}), mult({x}, {z}))
+    f>;
+    tprop Paxiom "Mul_distr_r" <f
+      forall x y z, [t] mult(plus({y}, {z}), {x}) = plus(mult({y}, {x}), mult({z}, {x}))
+    f>
+  ].
+
+(*Commutative Rings*)
+Definition MC_t_ts : typesym := mk_ts "MulComm.t" nil.
+Definition MC_t : vty := vty_cons MC_t_ts nil.
+Definition MC_op: funsym := binop "MulComm.op" MC_t.
+Definition CommutativeRing : theory :=
+  rev [
+    tclone Ring None nil nil nil;
+    tclone Comm (Some "MulComm") [(MC_t_ts, t_ts)] [(MC_op, mult)] nil
+  ].
+
+(*Commutative Rings With Unit*)
+Definition one : funsym := const "one" t.
+Definition UnitaryCommutativeRing : theory :=
+  rev [
+    tclone CommutativeRing None nil nil nil;
+    tdef (abs_fun one);
+    tprop Paxiom "Unitary" <f forall x, [t] mult(one(), {x}) = {x} f>;
+    tprop Paxiom "NonTrivialRing" <f not ([t] zero() = one()) f>
+  ].
+
+(*Ordered Commutative Rings*)
+(*TODO: need to do Relations and Orders - good because we 
+  can do some inductive predicates
+  start with this*)
+
+End Algebra.
