lib/Verif_Algebra.v
@@ -1,0 +1,106 @@
+Require Import Tactics.
+Require Import Algebra.
+
+(*All of the "valid_theory" proofs are trivial; there is just typing info to check
+  because there are only axioms*)
+
+(*Associativity*)
+Lemma assoc_typed : typed_theory Algebra.Assoc.
+Proof.
+  check_theory. 
+Qed.
+Lemma assoc_valid: valid_theory Algebra.Assoc.
+Proof.
+  simpl. split; auto. prove_axiom_wf.
+Qed.
+
+(*Commutativity*)
+Lemma comm_typed : typed_theory Algebra.Comm.
+Proof.
+  check_theory. 
+Qed.
+Lemma comm_valid: valid_theory Algebra.Comm.
+Proof.
+  simpl. split; auto. prove_axiom_wf.
+Qed.
+
+
+(*Associativity and Commutativity*)
+Lemma AC_typed : typed_theory Algebra.AC.
+Proof.
+  check_theory. 
+Qed.
+Lemma AC_valid: valid_theory Algebra.AC.
+Proof.
+  simpl. auto. 
+Qed.
+
+(*Monoids*)
+Lemma monoid_typed : typed_theory Algebra.Monoid.
+Proof.
+  check_theory. 
+Qed.
+Lemma monoid_valid: valid_theory Algebra.Monoid.
+Proof.
+  simpl. split; auto. prove_axiom_wf.
+Qed.
+
+(*Commutative monoids*)
+Lemma comm_monoid_typed : typed_theory Algebra.CommutativeMonoid.
+Proof.
+  check_theory. 
+Qed.
+Lemma comm_monoid_valid: valid_theory Algebra.CommutativeMonoid.
+Proof.
+  simpl. auto.
+Qed.
+
+(*Groups*)
+Lemma group_typed : typed_theory Algebra.Group.
+Proof.
+  check_theory. 
+Qed.
+Lemma group_valid: valid_theory Algebra.Group.
+Proof.
+  simpl. repeat(split; [prove_axiom_wf| auto]). 
+Qed.
+
+(*Commutative groups*)
+Lemma comm_group_typed : typed_theory Algebra.CommutativeGroup.
+Proof.
+  check_theory. 
+Qed.
+Lemma comm_group_valid: valid_theory Algebra.CommutativeGroup.
+Proof.
+  simpl. auto.
+Qed. 
+
+(*Rings*)
+Lemma ring_typed : typed_theory Algebra.Ring.
+Proof.
+  check_theory. 
+Qed.
+Lemma ring_valid: valid_theory Algebra.Ring.
+Proof.
+  simpl. repeat(split; [prove_axiom_wf| auto]). 
+Qed.
+
+(*Commutative Rings*)
+Lemma comm_ring_typed : typed_theory Algebra.CommutativeRing.
+Proof.
+  check_theory. 
+Qed.
+Lemma comm_ring_valid: valid_theory Algebra.CommutativeRing.
+Proof.
+  simpl. auto. 
+Qed.
+
+(*Commutative Rings With Unit*)
+Lemma comm_unitring_typed : typed_theory Algebra.UnitaryCommutativeRing.
+Proof.
+  check_theory. 
+Qed.
+Lemma comm_unitring_valid: valid_theory Algebra.UnitaryCommutativeRing.
+Proof.
+  simpl. repeat(split; [prove_axiom_wf| auto]).
+Qed.
